WIP fixing validity proof
Lots of additional lemmas on context_subst/subslet needed. Not being
paranoid in the typing relation renders this a bit harder than strictly necessary.

pcuic/theories/PCUICValidity.v
@@ -1,14 +1,163 @@
 From Coq Require Import Bool String List Program BinPos Compare_dec PeanoNat Lia.
-From MetaCoq.Template Require Import utils.
+From MetaCoq.Template Require Import utils UnivSubst.
 From MetaCoq.PCUIC Require Import PCUICAst PCUICAstUtils PCUICInduction
      PCUICLiftSubst PCUICTyping PCUICWeakeningEnv PCUICWeakening PCUICInversion
-     PCUICSubstitution PCUICReduction PCUICCumulativity PCUICGeneration.
+     PCUICSubstitution PCUICReduction PCUICCumulativity PCUICGeneration PCUICParallelReductionConfluence
+     PCUICConfluence
+     PCUICUnivSubst.
+
 From Equations Require Import Equations.
 Require Import ssreflect.
 Existing Instance config.default_checker_flags.
 
 Derive NoConfusion for term.
 Derive Signature for typing cumul.
+
+Lemma context_assumptions_subst_instance_context u Γ :
+  context_assumptions (subst_instance_context u Γ) = context_assumptions Γ.
+Proof.
+  induction Γ as [|[na [b|] ty] Γ]; simpl; auto.
+Qed.
+
+Lemma red_ctx_red Σ Γ Γ' t u :
+  red Σ Γ t u ->
+  (* red_ctx Σ Γ Γ' -> *)
+  red Σ Γ' t u.
+Proof. Admitted.
+
+Lemma invert_red_sort Σ Γ u v :
+  red Σ Γ (tSort u) v -> v = tSort u.
+Proof.
+  intros H; apply red_alt in H.
+  depind H. depind r. solve_discr.
+  reflexivity.
+  eapply IHclos_refl_trans2. f_equal. auto.
+Qed.
+
+Lemma invert_red_prod Σ Γ na A B v : wf Σ ->
+  red Σ Γ (tProd na A B) v ->
+  ∑ A' B', (v = tProd na A' B') *
+           (red Σ Γ A A') *
+           (red Σ (vass na A :: Γ) B B').
+Proof.
+  intros wfΣ H. apply red_alt in H.
+  depind H.
+  depelim r. solve_discr.
+  do 2 eexists. repeat split; eauto with pcuic.
+  do 2 eexists. repeat split; eauto with pcuic.
+  do 2 eexists. repeat split; eauto with pcuic.
+  destruct IHclos_refl_trans1 as (? & ? & (-> & ?) & ?). auto.
+  specialize (IHclos_refl_trans2 _ _ _ _ wfΣ eq_refl).
+  destruct IHclos_refl_trans2 as (? & ? & (-> & ?) & ?).
+  do 2 eexists. repeat split; eauto with pcuic.
+  now transitivity x.
+  transitivity x0; auto.
+  eapply red_red_ctx. eauto. eauto.
+  constructor. admit. red. auto.
+Admitted.
+
+Derive Signature for eq_term_upto_univ.
+
+Lemma red_conv (Σ : global_context) Γ t u : red Σ Γ t u -> Σ ;;; Γ |- t = u.
+Proof.
+  intros. now eapply conv_conv_alt, red_conv_alt.
+Qed.
+
+Lemma conv_cumul Σ Γ t u :
+  Σ ;;; Γ |- t = u -> (Σ ;;; Γ |- t <= u) * (Σ ;;; Γ |- u <= t).
+Proof. trivial. Qed.
+
+Lemma conv_sym Σ Γ t u : Σ ;;; Γ |- t = u -> Σ ;;; Γ |- u = t.
+Proof.
+  intros. eapply conv_cumul in X. split; intuition auto.
+Qed.
+
+(* TODO from Inversion *)
+  Lemma conv_trans :
+    forall Σ Γ u v w,
+      Σ ;;; Γ |- u = v ->
+      Σ ;;; Γ |- v = w ->
+      Σ ;;; Γ |- u = w.
+  Proof.
+    intros Σ Γ u v w h1 h2.
+    destruct h1, h2. constructor ; eapply cumul_trans ; eassumption.
+  Qed.
+
+(* FIXME leq_term_upto_univ is wrong: it assumes le for domains of products *)
+Lemma invert_cumul_prod_r Σ Γ C na A B : wf Σ ->
+  Σ ;;; Γ |- C <= tProd na A B ->
+  ∑ na' A' B', red Σ Γ C (tProd na' A' B') *
+               (Σ ;;; Γ |- A = A') *
+               (Σ ;;; Γ |- B' <= B').
+Proof.
+  intros wfΣ Hprod.
+  eapply cumul_alt in Hprod as [v [v' [[redv redv'] leqvv']]].
+  eapply invert_red_prod in redv' as (A' & B' & ((-> & Ha') & ?)).
+  depelim leqvv'.
+  do 3 eexists; intuition eauto.
+  eapply conv_trans.
+  eapply red_conv. eauto.
+  eapply conv_sym. eapply conv_conv_alt.
+  constructor. red. apply leqvv'1. auto.
+Qed.
+
+Lemma invert_cumul_sort_r Σ Γ C u :
+  Σ ;;; Γ |- C <= tSort u ->
+  ∑ u', red Σ Γ C (tSort u') * leq_universe (snd Σ) u' u.
+Proof.
+  intros Hcum.
+  eapply cumul_alt in Hcum as [v [v' [[redv redv'] leqvv']]].
+  eapply invert_red_sort in redv' as ->.
+  depelim leqvv'. exists s. intuition eauto.
+Qed.
+
+Lemma red_confluence {Σ Γ t u v} : wf Σ ->
+  red Σ Γ t u -> red Σ Γ t v ->
+  ∃ v', red Σ Γ u v' * red Σ Γ v v'.
+Proof.
+  move=> wfΣ H H'. apply red_alt in H. apply red_alt in H'.
+  destruct (red1_confluent wfΣ _ _ _ _ H H') as [nf [redl redr]].
+  apply red_alt in redl; apply red_alt in redr.
+  exists nf; intuition auto.
+Qed.
+
+Lemma type_unicity_prod {Σ Γ t na na' A A' B B'} : wf Σ ->
+  Σ ;;; Γ |- t : tProd na A B ->
+  Σ ;;; Γ |- t : tProd na' A' B' ->
+  Σ ;;; Γ |- A = A'.
+Proof.
+  intros wfΣ X X0.
+  generalize (principal_typing _ X X0); move=> [C [HC1 [HC2 HtC]]].
+  eapply invert_cumul_prod_r in HC1 => //.
+  eapply invert_cumul_prod_r in HC2 => //.
+  destruct HC1 as [na0 [A0 [B0 [[HC0 HA0] HB0]]]].
+  destruct HC2 as [na1 [A1 [B1 [[HC1 HA1] HB1]]]].
+  (* Confluence needed *)
+  destruct (red_confluence wfΣ HC0 HC1) as [pitype [redl redr]].
+  eapply invert_red_prod in redl as (?&?&(?&?)&?) => //.
+  eapply invert_red_prod in redr as (?&?&(?&?)&?) => //.
+  subst. noconf e0.
+  eapply red_conv in r; eapply red_conv in r1.
+  eapply conv_sym in r1. eapply conv_trans; eauto.
+  eapply conv_trans; eauto.
+  eapply conv_trans; eauto. eapply conv_sym; eauto.
+Qed.
+
+Lemma type_unicity_discr_prod_sort {Σ Γ t na A B u} : wf Σ ->
+  Σ ;;; Γ |- t : tProd na A B ->
+  Σ ;;; Γ |- t : tSort u -> False.
+Proof.
+  intros wfΣ X X0.
+  generalize (principal_typing _ X X0); move=> [C [HC1 [HC2 HtC]]].
+  eapply invert_cumul_prod_r in HC1 => //.
+  eapply invert_cumul_sort_r in HC2 => //.
+  destruct HC1 as [na0 [A0 [B0 [[HC0 HA0] HB0]]]].
+  destruct HC2 as [u' [redu' lequ']].
+  (* Confluence needed *)
+  destruct (red_confluence wfΣ HC0 redu') as [reduct [redl redr]].
+  eapply invert_red_prod in redl as (?&?&(?&?)&?) => //.
+  eapply invert_red_sort in redr as ?. subst. discriminate.
+Qed.
 
 Lemma isWfArity_or_Type_lift Σ n Γ ty (isdecl : n <= #|Γ|):
   wf Σ -> wf_local Σ Γ ->
@@ -94,7 +243,7 @@ Proof.
   - left.
     exists ctx, s. split; pcuic.
 Admitted.
-Derive Signature for subslet.
+Derive Signature for subslet context_subst.
   Notation "'∑'  x .. y , P" := (sigT (fun x => .. (sigT (fun y => P%type)) ..))
     (at level 200, x binder, y binder, right associativity) : type_scope.
 Hint Constructors subslet : pcuic.
@@ -137,44 +286,511 @@ Proof.
       rewrite <- H0. constructor; auto. rewrite !subst_app_simpl in t0. now simpl in t0.
 Qed.
 
+Lemma subslet_app_inv Σ Γ args args' l l' :
+  (subslet Σ Γ args' l' * subslet Σ Γ args (subst_context args' 0 l)) ->
+  subslet Σ Γ (args ++ args') (l ++ l').
+Proof.
+  intros Hs. destruct Hs.
+  induction l in l', s, s0, args, args' |- *.
+  - simpl. now depelim s0.
+  - rewrite subst_context_snoc0 in s0.
+    pose proof (substlet_length s0). unfold snoc in H. simpl in H. rewrite subst_context_length in H.
+    depelim s0. hnf in H. noconf H.
+    + destruct a as [na [b|] ty]; noconf H.
+      cbn in *. constructor. apply IHl; auto. rewrite subst_app_simpl. simpl.
+      noconf H0. hnf in H. now rewrite H.
+    + destruct a as [na' [b|] ty]; hnf in H; noconf H.
+      cbn in *. noconf H0. hnf in H. rewrite -H.
+      rewrite -subst_app_simpl. constructor. auto.
+      now rewrite !subst_app_simpl H.
+Qed.
+
+Lemma context_assumptions_app Γ Γ' :
+  context_assumptions (Γ ++ Γ') = context_assumptions Γ + context_assumptions Γ'.
+Proof.
+  induction Γ as [|[na [b|] ty] tl]; simpl; auto.
+Qed.
+
+Lemma skipn_S {A} a (l : list A) n : skipn (S n) (a :: l) = skipn n l.
+Proof. reflexivity. Qed.
+
+Lemma context_assumptions_skipn n Γ :
+  context_assumptions (skipn n Γ) = context_assumptions Γ - context_assumptions (firstn n Γ).
+Proof.
+  induction n in Γ |- *; cbn.
+  - unfold skipn. lia.
+  - destruct Γ; trivial. rewrite skipn_S.
+    rewrite IHn. destruct c as [na [b|] ty]; simpl; auto.
+Qed.
+
+Derive Signature for le.
+
+Lemma firstn_app_eq {A} (l l' : list A) n : #|l| = n -> firstn n (l ++ l') = l.
+Proof.
+  induction l in l', n |- *; destruct n; simpl; auto. discriminate. discriminate.
+  intros H. now rewrite [firstn _ _]IHl.
+Qed.
+
+Lemma firstn_app_ge {A} (l l' : list A) n : #|l| <= n -> firstn n (l ++ l') = l ++ firstn (n - #|l|) l'.
+Proof.
+  induction l in l', n |- *; destruct n; simpl; auto.
+  intros. depelim H.
+  intros H. now rewrite [firstn _ _]IHl.
+Qed.
+
+Lemma firstn_app_lt {A} (l l' : list A) n : n <= #|l| -> firstn n (l ++ l') = firstn n l.
+Proof.
+  induction l in l', n |- *; destruct n; simpl; auto.
+  intros. depelim H. intros H.
+  now rewrite [firstn _ _]IHl.
+Qed.
+
+Lemma skipn_app_eq {A} (l l' : list A) n : #|l| = n -> skipn n (l ++ l') = l'.
+Proof.
+  induction l in l', n |- *; destruct n; simpl; auto. discriminate. discriminate.
+  intros H. now rewrite [skipn _ _]IHl.
+Qed.
+
+Lemma skipn_app_ge {A} (l l' : list A) n : #|l| <= n -> skipn n (l ++ l') = skipn (n - #|l|) l'.
+Proof.
+  induction l in l', n |- *; destruct n; simpl; auto.
+  intros. depelim H.
+  intros H. now rewrite [skipn _ _]IHl.
+Qed.
+
+Lemma skipn_app_lt {A} (l l' : list A) n : n <= #|l| -> skipn n (l ++ l') = skipn n l ++ l'.
+Proof.
+  induction l in l', n |- *; destruct n; simpl; auto.
+  intros. depelim H. intros H.
+  now rewrite [skipn _ _]IHl.
+Qed.
+
+Lemma context_assumptions_subst_context s n Γ :
+  context_assumptions (subst_context s n Γ) = context_assumptions Γ.
+Proof.
+  induction Γ as [|[? [?|] ?] ?]; rewrite ?subst_context_snoc; simpl; auto.
+Qed.
+
+Lemma firstn_length_inv {A} n (l : list A) : #|firstn n l| = n -> n <= #|l|.
+Proof.
+  induction n in l |- *; destruct l; simpl; try lia. simpl in IHn.
+  intros [=]. specialize (IHn _ H0). lia.
+Qed.
+
+Lemma context_subst_app Γ args s s' :
+  context_subst Γ args (s ++ s') <~>
+  context_subst (skipn #|s| Γ) (List.firstn (context_assumptions (skipn #|s| Γ)) args) s' *
+  context_subst (subst_context s' 0 (firstn #|s| Γ)) (List.skipn (context_assumptions (skipn #|s| Γ)) args) s.
+Proof.
+  split.
+  intros Hs. depind Hs.
+  - destruct s; simpl in *; try congruence. subst.
+    intros. split; constructor.
+  - rewrite firstn_app.
+    pose proof (context_subst_length _ _ _ Hs).
+    pose proof (context_subst_assumptions_length _ _ _ Hs).
+    destruct s0; noconf H; try (simpl in *; congruence).
+    + simpl context_assumptions. rewrite H1.
+      rewrite firstn_all2. lia.
+      rewrite Nat.sub_succ_l. lia. simpl. rewrite Nat.sub_diag. simpl.
+      split; try constructor; auto.
+      rewrite skipn_all2 ?app_length /=. lia. constructor.
+    + specialize (IHHs Γ _ s0 s' eq_refl). simpl. rewrite skipn_S.
+      destruct IHHs. rewrite app_length in H0.
+      rewrite -H1. rewrite {2}context_assumptions_skipn.
+      set (nth := context_assumptions _ - _ - _).
+      assert (nth = 0) as -> by (subst nth; lia).
+      simpl. rewrite app_nil_r. split; intuition auto.
+      rewrite skipn_app_lt.
+      rewrite context_assumptions_skipn. lia.
+      rewrite subst_context_snoc. now constructor.
+  - pose proof (context_subst_length _ _ _ Hs).
+    pose proof (context_subst_assumptions_length _ _ _ Hs).
+    destruct s0; noconf H; simpl in *; try congruence.
+    + specialize (IHHs Γ args [] s eq_refl) as [Hs' Hs''].
+      split; try constructor; auto.
+    + rewrite app_length in H0.
+      specialize (IHHs Γ _ s0 s' eq_refl) as [Hs' Hs''].
+      split; auto.
+      rewrite subst_context_snoc. simpl.
+      rewrite subst_app_simpl. rewrite Nat.add_0_r. simpl.
+      unfold subst_decl, map_decl. simpl. rewrite skipn_S.
+      rewrite firstn_length_le. lia.
+      now constructor.
+  - intros [H H'].
+    assert (#|args| = context_assumptions Γ).
+    { rewrite -{1}(firstn_skipn #|s| Γ) context_assumptions_app.
+      rewrite -{1}(firstn_skipn (context_assumptions (skipn #|s| Γ)) args) app_length.
+      rewrite -(context_subst_assumptions_length _ _ _ H).
+      rewrite -(context_subst_assumptions_length _ _ _ H').
+      rewrite context_assumptions_subst_context.
+      lia. }
+    induction s in Γ, args, s', H, H', H0 |- *; simpl in *.
+
+    unfold skipn in H. rewrite -H0 in H.
+    rewrite firstn_all2 in H. auto. auto.
+
+    destruct Γ; try discriminate.
+    simpl in *. destruct args; simpl in *; try discriminate. depelim H'.
+    destruct c as [na [b|] ty]. simpl in *.
+    + rewrite skipn_S in H, H'.
+      rewrite subst_context_snoc0 in H'.
+      unfold subst_decl, map_decl in H'. simpl in *.
+      specialize (IHs _ _ _ H). depelim H'. hnf in H1. noconf H1.
+      hnf in H1. noconf H1.
+      pose proof (subst_app_simpl s0 s' 0 b). simpl in H1.
+      rewrite firstn_length_le.
+      { move: (context_subst_length _ _ _ H').
+        rewrite subst_context_length.
+        now move/firstn_length_inv. }
+      rewrite -H1. constructor. apply IHs; auto.
+    + rewrite skipn_S in H, H'.
+      rewrite subst_context_snoc0 in H'.
+      unfold subst_decl, map_decl in H'. simpl in *.
+      destruct args using rev_ind; try discriminate.
+      rewrite app_length in H0. simpl in H0.
+      depelim H'. hnf in H0. noconf H0.
+      assert ((context_assumptions (skipn #|s| Γ)) <= #|args|).
+      { rewrite context_assumptions_skipn. lia. }
+      rewrite skipn_app_lt in H1. auto.
+      apply app_inj_tail in H1 as [<- ->].
+      constructor. apply IHs.
+      rewrite firstn_app in H.
+      assert (context_assumptions (skipn #|s| Γ) - #|args| = 0) by lia.
+      rewrite H1 in H. simpl in H. now rewrite app_nil_r in H.
+      auto. lia.
+      hnf in H0. noconf H0.
+Qed.
+
+Lemma typing_spine_tLetIn Σ Γ na b ty T args U :
+  typing_spine Σ Γ (T {0 := b}) args U ->
+  typing_spine Σ Γ (tLetIn na b ty T) args U.
+Proof.
+  intros Hs. depind Hs.
+  - constructor. auto. econstructor 2. constructor. auto.
+  - econstructor; eauto. econstructor 2. constructor. auto.
+Qed.
+
+Lemma firstn_none {A} n (l : list A) : n = 0 -> firstn n l = [].
+Proof. intros ->. destruct l; reflexivity. Qed.
+
+Lemma skipn_none {A} n (l : list A) : n = 0 -> skipn n l = l.
+Proof. intros ->. destruct l; reflexivity. Qed.
+
 Lemma typing_spine_arity Σ Γ ctx u args s :
   wf_local Σ Γ ->
   context_subst ctx args s ->
   subslet Σ Γ s ctx ->
+  wf_local Σ (Γ ,,, ctx) ->
   typing_spine Σ Γ (it_mkProd_or_LetIn ctx (tSort u)) args (tSort u).
 Proof.
-  intros wfΓ Hargss Hs. revert args Hargss Hs; induction ctx using rev_ind; cbn; intros.
-  - depelim Hs. depelim Hargss. constructor; auto. left. exists [], u. intuition auto.
-  - rewrite it_mkProd_or_LetIn_app. simpl.
-    destruct x as [na [b|] ty]; cbn.
-    + eapply subslet_app in Hs as (args' & args'' & (-> & H) & H').
-      depelim H. simpl in H0. noconf H0.
-      hnf in H0. noconf H0. depelim H. rewrite !subst_empty in t0, H', Hargss.
+  intros wfΓ Hargss Hs (* Hctx *). revert s args ctx Hargss Hs (* Hctx *). induction s using rev_ind; cbn; intros.
+  - depelim Hargss. constructor; auto. left. exists [], u. intuition auto.
+  - eapply context_subst_app in Hargss as [instna instl].
+    destruct ctx using rev_ind.
+    + simpl in *. rewrite skipn_nil in instna.
+      simpl in *. depelim instna.
+    + clear IHctx.
+      pose proof (substlet_length Hs). rewrite !app_length in H. simpl in H.
+      assert (#|s| = #|l|) by lia.
+      rewrite skipn_app_lt in instna. lia.
+      rewrite it_mkProd_or_LetIn_app. simpl.
+      rewrite firstn_app in instl.
+      rewrite [firstn (_ - _) _]firstn_none in instl. lia.
+      rewrite firstn_all2 in instl. lia.
+      rewrite app_nil_r in instl.
+      rewrite skipn_app_ge in instl. lia.
+      rewrite [skipn (_ - _) _]skipn_none in instl. lia.
+      rewrite skipn_all2 in instna. by lia.
+      destruct x0 as [na [b|] ty]. simpl in *.
+      ++ unfold mkProd_or_LetIn. simpl.
+         eapply typing_spine_tLetIn.
+         unfold subst1. rewrite subst_it_mkProd_or_LetIn.
+         simpl.
+         eapply subslet_app in Hs as (args' & args'' & (Heq & H') & H'').
+         depelim H'; hnf in H1; noconf H1. depelim H'.
+         rewrite !subst_empty in Heq, t0, H''.
+         eapply app_inj_tail in Heq as [<- <-].
+         depelim instna. destruct args0; discriminate. hnf in H1; noconf H1.
+         rewrite subst_empty in instl, H'', t0 |- *.
+         eapply IHs; eauto. simpl in H1. admit. (* provable wf_local *)
+      ++ unfold mkProd_or_LetIn. cbn.
+         eapply subslet_app in Hs as (args' & args'' & (Heq & H') & H'').
+         depelim H'; hnf in H1; noconf H1. depelim H'.
+         rewrite !subst_empty in Heq, t0, H''.
+         eapply app_inj_tail in Heq as [<- <-]. simpl in *.
+         destruct args. depelim instna; hnf in H1; noconf H1.
+         destruct args; discriminate.
+         depelim instna; hnf in H1; noconf H1. depelim instna. noconf H2.
+         rewrite skipn_S in instl. unfold skipn in instl.
+         econstructor; eauto. left.
+         exists (l ++ [vass na ty]), u. simpl.
+         rewrite destArity_it_mkProd_or_LetIn. simpl. split; auto.
+         rewrite /subst1 subst_it_mkProd_or_LetIn /=.
+         eapply IHs; eauto.
+         admit. (* provable wf_local *)
 Admitted.
 
-(* Lemma invert_type_mkApps Σ Γ f u T fty : *)
-(*   Σ ;;; Γ |- mkApps f u : T -> *)
-(*   isWfArity typing Σ Γ T -> *)
-(*   Σ ;;; Γ |- f : fty -> *)
-(*   typing_spine Σ Γ fty u T. *)
+(* Lemma typing_spine_arity Σ Γ ctx s args : *)
+(*   wf_local Σ Γ -> *)
+(*   subslet Σ Γ args ctx -> *)
+(*   typing_spine Σ Γ (it_mkProd_or_LetIn ctx (tSort s)) args (tSort s). *)
 (* Proof. *)
-(*   induction u in f, T |- *; simpl. *)
-(*   - intros HT HwfT Hf. constructor. left; auto. eapply cumul_refl'. *)
-(*   - intros Hf Hty. *)
-(*     specialize (IHu _ _ Hf Hty) as [T' [Hwfa Hf']]. *)
-(*     red in Hty. destruct Hty as [ctx [s [Hd Hwf]]]. *)
-(*     generalize (PCUICClosed.destArity_spec [] T). rewrite Hd. *)
-(*     simpl. intros ->. clear Hd. *)
-(*     (* red in Hwfa. destruct Hwfa as [ctx' [s' [Hd' Hwf']]]. *) *)
-(*     (* generalize (PCUICClosed.destArity_spec [] T'). rewrite {}Hd'. *) *)
-(*     (* simpl. intros ->. *) *)
-(*     eapply inversion_App in Hwfa as (fna & fA & fB & Hfp & Hfa & Hf''). *)
-(*     exists (tProd fna fA fB). intuition auto. *)
-(*     econstructor. 2:eapply cumul_refl'. admit. *)
-(*     auto. *)
-(*   exists T', U'. split; auto. split; auto. *)
-(*   eapply cumul_trans; eauto. *)
-(* Qed. *)
+(*   intros wfΓ Hs. revert args Hs; induction ctx using rev_ind; cbn; intros. *)
+(*   - depelim Hs. constructor; auto. left. exists [], s. intuition auto. *)
+(*   - rewrite it_mkProd_or_LetIn_app. simpl. *)
+(*     destruct x as [na [b|] ty]; cbn. *)
+(*     eapply subslet_app in Hs as (args' & args'' & (-> & H) & H'). *)
+(*     depelim H. simpl in H0. noconf H0. *)
+(*     hnf in H0. noconf H0. depelim H. rewrite subst_empty. *)
+(*     rewrite subst_empty in H'. simpl in H'. *)
+
+
+
+(*     depelim Hs. apply (f_equal (@length _)) in H. rewrite app_length in H. simpl in H; elimtype False. lia. *)
+
+(*     eapply (type_spine_cons Σ Γ t s0 na T). econstructor. 3:eauto. *)
+
+
+
+Lemma invert_type_mkApps_head Σ Γ f s u :
+  Σ ;;; Γ |- mkApps f u : tSort s ->
+  ∑ T, Σ ;;; Γ |- f : T.
+Proof.
+  induction u in f |- *; simpl; move=> Hf.
+  exists (tSort s). auto.
+  destruct (IHu (tApp f a) Hf).
+  eapply inversion_App in t as (fna & fA & fB & Hfp & Hfa & Hf'').
+  eexists ; eauto.
+Qed.
+
+(* Lemma invert_type_mkApps Σ Γ f ctx s u : *)
+(*   (* If the head's type is syntactically an arity *) *)
+(*   Σ ;;; Γ |- f : it_mkProd_or_LetIn ctx (tSort s) -> *)
+(*   #|u| = context_assumptions ctx -> *)
+(*   (* An the application is well-typed *) *)
+(*   Σ ;;; Γ |- mkApps f u : tSort s -> *)
+(*   (* We can extract another typing of the head and show that the arguments are a well-typed *)
+(*      substitution for it *) *)
+(*   ∑ ctx' subs, (Σ ;;; Γ |- f : it_mkProd_or_LetIn ctx' (tSort s)) * *)
+(*                (context_subst ctx' u subs * subslet Σ Γ subs ctx')%type. *)
+(* Proof. *)
+(*   (* induction u in f, ctx |- *; cbn. *) *)
+(*   Subterm.rec_wf_rel IH #|ctx| lt. simpl. *)
+(*   rename pr1 into Σ. *)
+(*   rename pr0 into Γ. *)
+(*   rename pr2 into t. *)
+(*   rename pr3 into ctx. *)
+(*   rename pr4 into s. *)
+(*   rename pr5 into u. clear H1. *)
+(*   destruct ctx as [|[na [b|] ty] ctx] using rev_ind; move=> /= Hf Hu Hfu. *)
+(*   - exists [], []. split; auto; try constructor. *)
+(*     destruct u; noconf Hu. constructor. constructor. *)
+(*   - clear IHctx. rewrite context_assumptions_app in Hu. simpl in Hu. *)
+(*     rewrite it_mkProd_or_LetIn_app in Hf. *)
+(*     cbn in Hf. *)
+(*     specialize (IH Σ Γ t (subst_context [b] 0 ctx) s u). *)
+(*     rewrite app_length subst_context_length in IH. cbn in IH. *)
+(*     forward IH by lia. *)
+(*     forward IH. *)
+(*     { eapply type_Conv. eauto. admit. *)
+(*       econstructor 2. constructor. *)
+(*       now rewrite /subst1 subst_it_mkProd_or_LetIn. } *)
+(*     forward IH. *)
+(*     { rewrite context_assumptions_subst_context. lia. } *)
+(*     specialize (IH Hfu) as [ctx' [s' [tctx' [ctxs subsl]]]]. *)
+(*     exists ctx', s'. *)
+(*     split; auto. *)
+(*   - clear IHctx. rewrite context_assumptions_app in Hu. simpl in Hu. *)
+(*     rewrite it_mkProd_or_LetIn_app in Hf. *)
+(*     cbn in Hf. *)
+(*     destruct u as [|a u]. simpl in Hu. elimtype False. lia. *)
+(*     simpl in Hu. *)
+(*     specialize (IH Σ Γ (tApp t a) (subst_context [a] 0 ctx) s u). *)
+(*     rewrite app_length subst_context_length in IH. cbn in IH. *)
+(*     forward IH by lia. *)
+(*     forward IH. *)
+(*     { eapply refine_type. eapply type_App. eauto. *)
+(*       cbn in Hfu. eapply invert_type_mkApps_head in Hfu. *)
+(*       destruct Hfu as [appty Happ]. *)
+(*       eapply inversion_App in Happ as (fna & fA & fB & Hfp & Hfa & Hf''). *)
+(*       pose proof (type_unicity_prod Hf Hfp). eapply type_Conv. eauto. admit. *)
+(*       eapply X. *)
+(*       now rewrite /subst1 subst_it_mkProd_or_LetIn. } *)
+(*     forward IH. *)
+(*     { rewrite context_assumptions_subst_context. lia. } *)
+(*     specialize (IH Hfu) as [ctx' [s' [ctxs subsl]]]. *)
+(*     exists (ctx ++ [vass na ty]), (s' ++ [a]). *)
+(*     split; auto. now rewrite it_mkProd_or_LetIn_app. *)
+(*     split. *)
+(*     admit. *)
+(*     admit. *)
+(* Admitted. *)
+(* Set SimplIsCbn. *)
+
+Lemma destArity_Let {Γ na b b_ty t_ty ctx s} :
+  destArity Γ (tLetIn na b b_ty t_ty) = Some (ctx, s) ->
+  destArity Γ (t_ty {0 := b}) =
+  let pos := #|ctx| - #|Γ| in
+  Some (subst_context [b] 0 (List.firstn (Nat.pred pos) ctx) ++ List.skipn pos ctx, s).
+Proof.
+  simpl. intros.
+  pose proof (PCUICClosed.destArity_spec (Γ ,, vdef na b b_ty) t_ty). rewrite H in H0.
+  simpl in H0.
+Admitted.
+
+Lemma type_LetIn_red Σ Γ t na b b_ty t_ty :
+  isWfArity typing Σ Γ (tLetIn na b b_ty t_ty) ->
+  Σ ;;; Γ |- t : tLetIn na b b_ty t_ty ->
+  Σ ;;; Γ |- t : t_ty {0 := b}.
+Proof.
+  intros.
+  eapply type_Conv; eauto.
+  left. red. red in X. destruct X as [ctx [s [dAr wfl]]].
+  exists (subst_context [b] 0 (List.firstn (Nat.pred #|ctx|) ctx)), s.
+  admit.
+  econstructor 2. constructor. eapply cumul_refl'.
+Admitted.
+
+Lemma invert_type_mkApps_args {Σ Γ f ctx s u} : wf Σ ->
+  Σ ;;; Γ |- f : it_mkProd_or_LetIn ctx (tSort s) ->
+  isWfArity typing Σ Γ (it_mkProd_or_LetIn ctx (tSort s)) ->
+  Σ ;;; Γ |- mkApps f u : tSort s ->
+  #|u| = context_assumptions ctx.
+Proof.
+  induction u in f, ctx |- *; simpl; auto.
+  intros.
+  Subterm.rec_wf_rel IH #|ctx| lt. simpl.
+  rename pr1 into Σ.
+  rename pr0 into Γ.
+  rename pr2 into t.
+  rename pr3 into ctx.
+  rename pr4 into s.
+  rename pr5 into wfΣ.
+  rename pr6 into Ht.
+  rename pr8 into Ht'. clear H0.
+  destruct ctx as [|[na [b|] ty] ctx] using rev_ind; cbn; eauto.
+  - rewrite it_mkProd_or_LetIn_app in Ht. cbn in Ht.
+    eapply type_LetIn_red in Ht.
+    rewrite context_assumptions_app. simpl. rewrite Nat.add_0_r.
+    rewrite /subst1 subst_it_mkProd_or_LetIn in Ht. simpl in Ht.
+    rewrite -(context_assumptions_subst_context [b] 0 ctx).
+    eapply IH. eauto. eauto. admit. eapply Ht'.
+    rewrite subst_context_length app_length /=. lia.
+    rewrite it_mkProd_or_LetIn_app in pr7. eapply pr7.
+
+  - rewrite it_mkProd_or_LetIn_app /= in pr7 Ht.
+    rewrite context_assumptions_app /=.
+    clear -wfΣ Ht Ht'. simpl in Ht.
+    now elim (type_unicity_discr_prod_sort wfΣ Ht Ht').
+
+  - intros.
+    destruct ctx as [|[na [b|] ty] ctx] using rev_ind; cbn; eauto.
+    + simpl in *.
+      eapply invert_type_mkApps_head in X2 as [T' HT'].
+      eapply inversion_App in HT' as [na [A' [B' [Hf' _]]]].
+      now elim (type_unicity_discr_prod_sort X Hf' X0).
+    + rewrite context_assumptions_app. simpl. rewrite Nat.add_0_r.
+      rewrite it_mkProd_or_LetIn_app in X X0. simpl in X, X0.
+Admitted.
+
+Lemma invert_type_mkApps {Σ Γ f ctx s} : wf Σ ->
+  Σ ;;; Γ |- f : it_mkProd_or_LetIn ctx (tSort s) ->
+  forall u, #|u| = context_assumptions ctx ->
+  Σ ;;; Γ |- mkApps f u : tSort s ->
+  { s & (context_subst ctx u s * subslet Σ Γ s ctx)%type }.
+Proof.
+  (* induction u in f, ctx |- *; cbn. *)
+  Subterm.rec_wf_rel IH #|ctx| lt. simpl.
+  rename pr1 into Σ.
+  rename pr0 into Γ.
+  rename pr2 into t.
+  rename pr3 into ctx.
+  rename pr4 into s.
+  clear H0. intros wfΣ.
+  destruct ctx as [|[na [b|] ty] ctx] using rev_ind; move=> /= Hf u Hu Hfu.
+  - exists []. split; auto; try constructor.
+    destruct u; noconf Hu. constructor.
+  - clear IHctx. rewrite context_assumptions_app in Hu. simpl in Hu.
+    rewrite it_mkProd_or_LetIn_app in Hf.
+    cbn in Hf.
+    specialize (IH Σ Γ t (subst_context [b] 0 ctx) s).
+    rewrite app_length subst_context_length in IH. cbn in IH.
+    forward IH by lia.
+    forward IH by auto.
+    forward IH.
+    { eapply type_Conv. eauto. admit.
+      econstructor 2. constructor.
+      now rewrite /subst1 subst_it_mkProd_or_LetIn. }
+    specialize (IH u).
+    forward IH.
+    { rewrite context_assumptions_subst_context. lia. }
+    specialize (IH Hfu) as [s' [ctxs subsl]].
+    exists (s' ++ [b]).
+    split; auto.
+    + eapply context_subst_app.
+      move:(context_subst_length _ _ _ ctxs). rewrite subst_context_length; move=> <-.
+      split.
+      ++ rewrite skipn_app_eq //. simpl. rewrite -{2}(subst_empty 0 b).
+         now repeat constructor.
+      ++ rewrite skipn_app_eq // firstn_app_eq //.
+    + eapply subslet_app_inv; split; auto.
+      pose proof (cons_let_def Σ Γ [] [] na b ty).
+      rewrite !subst_empty in X. eapply X. constructor. admit. (* Wf arity *)
+
+  - clear IHctx. rewrite context_assumptions_app in Hu. simpl in Hu.
+    rewrite it_mkProd_or_LetIn_app in Hf.
+    cbn in Hf.
+    destruct u as [|a u]. simpl in Hu. elimtype False. lia.
+    simpl in Hu.
+    specialize (IH Σ Γ (tApp t a) (subst_context [a] 0 ctx) s).
+    rewrite app_length subst_context_length in IH. cbn in IH.
+    forward IH by lia.
+    forward IH by auto.
+    forward IH.
+    { eapply refine_type. eapply type_App. eauto.
+      cbn in Hfu. eapply invert_type_mkApps_head in Hfu.
+      destruct Hfu as [appty Happ].
+      eapply inversion_App in Happ as (fna & fA & fB & Hfp & Hfa & Hf'').
+      pose proof (type_unicity_prod wfΣ Hf Hfp). eapply type_Conv. eauto. admit.
+      eapply X.
+      now rewrite /subst1 subst_it_mkProd_or_LetIn. }
+    specialize (IH u). forward IH.
+    { rewrite context_assumptions_subst_context. lia. }
+    specialize (IH Hfu) as [s' [ctxs subsl]].
+    exists (s' ++ [a]).
+    split; auto.
+    + eapply (context_subst_app (ctx ++ _) (a :: u) s' [a]).
+      move:(context_subst_length _ _ _ ctxs). rewrite subst_context_length; move=> <-.
+      simpl. split.
+      rewrite skipn_app_eq //. cbn.
+      apply (context_subst_ass [] [] [] na ty a). constructor.
+      rewrite firstn_app_eq // skipn_app_eq //.
+    + eapply subslet_app_inv. split; auto. constructor. constructor. rewrite subst_empty.
+      { cbn in Hfu. eapply invert_type_mkApps_head in Hfu.
+        destruct Hfu as [appty Happ].
+        eapply inversion_App in Happ as (fna & fA & fB & Hfp & Hfa & Hf'').
+        pose proof (type_unicity_prod wfΣ Hf Hfp). eapply type_Conv. eauto. admit.
+        eapply X. }
+Admitted.
+
+Definition infix_app {A B} (f : A -> B) (x : A) := f x.
+Infix "$" := infix_app (at level 20, right associativity).
+
+Lemma invert_mkApps_tInd {Σ Γ ind u args s} (wfΣ : wf Σ) :
+  Σ ;;; Γ |- mkApps (tInd ind u) args : tSort s ->
+  ∑ mdecl idecl (isdecl : declared_inductive (fst Σ) mdecl ind idecl),
+    let (onmind, onind) := on_declared_inductive wfΣ isdecl in
+    (#|args| = context_assumptions (ind_params mdecl ++ ind_indices onind)) *
+    leq_universe (snd Σ) (UnivSubst.subst_instance_univ u (ind_sort onind)) s *
+    (Σ ;;; Γ |- tInd ind u :
+    (subst_instance_constr u
+       $ it_mkProd_or_LetIn (ind_params mdecl)
+       $ it_mkProd_or_LetIn (ind_indices onind)
+       $ (tSort (ind_sort onind)))).
+Proof.
+  intros H.
+Admitted.
 
 Theorem validity :
   env_prop (fun Σ Γ t T => isWfArity_or_Type Σ Γ T).
@@ -291,7 +907,7 @@ Proof.
       subst ctx.
       pose proof (PCUICClosed.destArity_spec [] pty). rewrite Heq in H.
       simpl in H. subst pty.
-      assert (#|args| = #|pctx|). admit. (* WF of case *)
+      (* assert (#|args| = #|pctx|). admit. (* WF of case *) *)
       eapply type_mkApps. eauto.
       destruct X4. destruct i as [ctx' [s' [Heq' Hs']]].
       elimtype False.
@@ -304,9 +920,52 @@ Proof.
         intros. unshelve eapply (IHargs _ _ Heq').
         reflexivity. }
       destruct i as [si Hi].
+      destruct (invert_mkApps_tInd wfΣ Hi) as [mdecl' [idecl' [isdecl' Hi']]].
+      destruct on_declared_inductive as [onmind onib]; auto.
+      destruct Hi' as [[Hargs Hsorts] Hind].
+      (* rewrite !PCUICUnivSubst.subst_instance_constr_it_mkProd_or_LetIn in X1. *)
+      (* simpl in X1. *)
+      (* unfold types_of_case in heq_types_of_case. *)
+      (* destruct instantiate_params eqn:Heqinst; noconf heq_types_of_case. *)
+      (* destruct destArity as [[args' s']|] eqn:heq_dest; noconf heq_types_of_case. *)
+      (* rewrite destArity_it_mkProd_or_LetIn in heq_types_of_case. simpl in heq_types_of_case. *)
+      (* destruct map_option_out; noconf heq_types_of_case. *)
+      (* clear H. *)
+      (* rewrite ind_arity_eq in Heqinst. *)
+      (* eapply instantiate_params_make_context_subst in Heqinst. *)
+      (* destruct Heqinst as [ctx' [ty'' [s'' [Hdecomp [Hs'' Ht]]]]]. *)
+      (* rewrite decompose_prod_n_assum_it_mkProd app_nil_r in Hdecomp. *)
+      (* noconf Hdecomp. subst t. *)
+      (* eapply make_context_subst_spec in Hs''. *)
+      (* rewrite List.rev_involutive in Hs''. *)
+      (* rewrite subst_it_mkProd_or_LetIn /= destArity_it_mkProd_or_LetIn /= in heq_dest. *)
+      (* noconf heq_dest. rewrite app_context_nil_l. *)
+      (* rewrite destArity_it_mkProd_or_LetIn in heq_types_of_case. simpl in heq_types_of_case. *)
+      unfold infix_app in Hind. rewrite !subst_instance_constr_it_mkProd_or_LetIn in Hind.
+      rewrite -it_mkProd_or_LetIn_app in Hind.
+      simpl in Hind.
       admit.
       (* eapply (invert_type_mkApps _ _ (tInd ind u)) in Hi; pcuic. *)
       (* 2:{ econstructor; eauto. admit. (* universes *) } *)
+      (* 2:{ admit. } *)
+      (* (* Looks ok *) *)
+      (* admit. *)
+
+      (* pose proof (invert_type_mkApps Hind args). *)
+      (* rewrite !context_assumptions_app !context_assumptions_subst_instance_context in X1 Hargs. *)
+      (* forward X1 by lia. *)
+      (* forward X1. eapply type_Conv. *)
+      (* eauto. left. red. eexists [], _. split; try reflexivity. auto with pcuic. *)
+      (* constructor. constructor. *)
+
+
+
+
+
+      (* eapply typing_spine_arity. auto. *)
+      (* rewrite -(List.rev_involutive pctx). *)
+      (* eapply make_context_subst_spec. *)
+
       (* 2:{ admit. } *)
       (* (* Looks ok *) *)
       (* admit. *)
